Renamings.

Bmethod.thy
@@ -35,31 +35,31 @@ qed
 
 section {* B refinement: two components glued by a relation between states *}
 
-record REFINEMENT =
+record B_refinement =
   abstract :: LTS
   concrete :: LTS
-  invariant :: "STATE \<times> STATE \<Rightarrow> bool" (* relates Abstract to Concrete - see wd_REFINEMENT_glue *)
+  invariant :: "STATE \<times> STATE \<Rightarrow> bool" (* relates Abstract to Concrete - see wd_B_refinement_glue *)
   
-definition sound_REFINEMENT :: "REFINEMENT \<Rightarrow> bool" where
-"sound_REFINEMENT r \<equiv> lts_simulation {(s, s') | s s' . (invariant r) (s, s') } (concrete r) (abstract r)"
+definition sound_B_refinement :: "B_refinement \<Rightarrow> bool" where
+"sound_B_refinement r \<equiv> lts_simulation {(s, s') | s s' . (invariant r) (s, s') } (concrete r) (abstract r)"
 
 text {* A special refinement is one that does not change anything, namely the
 identity refinement. It is defined as a function that takes a machine and
 returns the identity refinement. *}
 
-definition refinement_id :: "LTS \<Rightarrow> REFINEMENT" where
+definition refinement_id :: "LTS \<Rightarrow> B_refinement" where
 "refinement_id m \<equiv> \<lparr> abstract = m, concrete = m, invariant = (\<lambda> p . fst p = snd p) \<rparr>"
 
 text {* We have that the identity refinement is sound. *}
 
-lemma "sound_REFINEMENT(refinement_id m)"
+lemma "sound_B_refinement(refinement_id m)"
 sorry
 
 text {* Next, we definement composition of refinements. This is only defined if the
 composed refinements have matching set of states, otherwise it is left
 undefined. *}
 
-definition refinement_compose :: "REFINEMENT \<Rightarrow> REFINEMENT \<Rightarrow> REFINEMENT option" where
+definition refinement_compose :: "B_refinement \<Rightarrow> B_refinement \<Rightarrow> B_refinement option" where
 "refinement_compose r1 r2 \<equiv> 
   (if concrete r1 = abstract r2 then
   Some \<lparr> abstract = abstract r1, concrete = concrete r2, invariant = \<lambda> p . \<exists> s . (invariant r1)(fst p, s) \<and> (invariant r2)(s, snd p)\<rparr>
@@ -67,9 +67,9 @@ definition refinement_compose :: "REFINEMENT \<Rightarrow> REFINEMENT \<Rightarr
 
 lemma refinement_compose_soundness:
   assumes 
-    "sound_REFINEMENT r1" and "sound_REFINEMENT r2" and
+    "sound_B_refinement r1" and "sound_B_refinement r2" and
     "refinement_compose r1 r2 = Some r"
-  shows "sound_REFINEMENT r"
+  shows "sound_B_refinement r"
 proof(cases "concrete r1 = abstract r2")
   case False
     hence "refinement_compose r1 r2 = None" by (simp add:refinement_compose_def)
@@ -79,7 +79,7 @@ proof(cases "concrete r1 = abstract r2")
 next
   case True
   assume "concrete r1 = abstract r2"
-  show "sound_REFINEMENT r" unfolding sound_REFINEMENT_def lts_simulation_def lts_simulation_init_def lts_simulation_transition_def
+  show "sound_B_refinement r" unfolding sound_B_refinement_def lts_simulation_def lts_simulation_init_def lts_simulation_transition_def
   sorry
 qed
 (*
@@ -90,11 +90,11 @@ qed
     with assms(3)
       have r: "r = rv" by simp
     from assms(2)
-      have i2: "sound_REFINEMENT_init r2" by (simp add: sound_REFINEMENT_def)
+      have i2: "sound_B_refinement_init r2" by (simp add: sound_B_refinement_def)
     from assms(1)
-      have i1: "sound_REFINEMENT_init r1" by (simp add: sound_REFINEMENT_def)    
+      have i1: "sound_B_refinement_init r1" by (simp add: sound_B_refinement_def)    
     from i2 and i1
-      have i: "sound_REFINEMENT_init rv" unfolding sound_REFINEMENT_init_def rv_def
+      have i: "sound_B_refinement_init rv" unfolding sound_B_refinement_init_def rv_def
     proof -
       have "\<forall>s\<in>init (concrete r2). \<exists>sa\<in>init (abstract r2). (invariant r2) (s, sa) \<Longrightarrow>
             \<forall>s\<in>init (abstract r2). \<exists>sa\<in>init (abstract r1). (invariant r1) (s, sa) \<Longrightarrow> 
@@ -112,12 +112,12 @@ qed
     qed
   moreover  
     from assms(1)
-      have t1: "sound_REFINEMENT_trans r1" by (simp add: sound_REFINEMENT_def)
+      have t1: "sound_B_refinement_trans r1" by (simp add: sound_B_refinement_def)
     from assms(2)
-      have t2: "sound_REFINEMENT_trans r2" by (simp add: sound_REFINEMENT_def)
+      have t2: "sound_B_refinement_trans r2" by (simp add: sound_B_refinement_def)
     from t1 and t2
-      have t: "sound_REFINEMENT_trans rv"
-      proof (simp add:sound_REFINEMENT_trans_def rv_def)
+      have t: "sound_B_refinement_trans rv"
+      proof (simp add:sound_B_refinement_trans_def rv_def)
         have 
           "\<forall>tc\<in>Trans (Concrete r1). \<exists>ta\<in>Trans (Abstract r1). (Src tc, Src ta) \<in> Glue r1 \<and> (Dst tc, Dst ta) \<in> Glue r1 \<and> Evt tc = Evt ta \<Longrightarrow>
            \<forall>tc\<in>Trans (Concrete r2). \<exists>ta\<in>Trans (Concrete r1). (Src tc, Src ta) \<in> Glue r2 \<and> (Dst tc, Dst ta) \<in> Glue r2  \<and> Evt tc = Evt ta \<Longrightarrow>
@@ -133,39 +133,39 @@ qed
           by simp
       qed
   ultimately
-    have "sound_REFINEMENT rv" 
-      by (simp add:sound_REFINEMENT_def)
-    with r show "sound_REFINEMENT r" by simp
+    have "sound_B_refinement rv" 
+      by (simp add:sound_B_refinement_def)
+    with r show "sound_B_refinement r" by simp
 qed
  *)
 text {* We now want to verify that our definition of refinement composition satisfies
 some simple properties. First any identity refinement is left-neutral: *}
 
 lemma refinement_compose_neutral_left:
-  assumes "sound_REFINEMENT r"
+  assumes "sound_B_refinement r"
   shows "abstract r = m \<Longrightarrow> refinement_compose (refinement_id m) r = Some r"
-proof(simp add:sound_REFINEMENT_def refinement_compose_def refinement_id_def)
+proof(simp add:sound_B_refinement_def refinement_compose_def refinement_id_def)
 qed
 
 text {* Second, any identity refinement is right-neutral for refinement composition. *}
 
 lemma refinement_compose_neutral_right:
-  assumes "sound_REFINEMENT r"
+  assumes "sound_B_refinement r"
   shows "concrete r = m \<Longrightarrow> refinement_compose r (refinement_id m) = Some r"
-proof(simp add:sound_REFINEMENT_def refinement_compose_def refinement_id_def)
+proof(simp add:sound_B_refinement_def refinement_compose_def refinement_id_def)
 qed
 
 text {* Last, refinement composition is associative. The expression of this
 property is not as straightforward as we could expect due to the partialness
 of composition. *}
 lemma refinement_compose_associative:
-  assumes "sound_REFINEMENT r1 \<and> sound_REFINEMENT r2 \<and> sound_REFINEMENT r3"
+  assumes "sound_B_refinement r1 \<and> sound_B_refinement r2 \<and> sound_B_refinement r3"
       and "concrete r1 = abstract r2" 
       and "concrete r2 = abstract r3"
   shows "\<exists> r12 r23 . Some r12 = refinement_compose r1 r2 \<and> 
          Some r23 = refinement_compose r2 r3 \<and>
          refinement_compose r12 r3 = refinement_compose r1 r23"
-proof(simp add:sound_REFINEMENT_def refinement_compose_def, auto)
+proof(simp add:sound_B_refinement_def refinement_compose_def, auto)
   from assms(2) show "concrete r1 = abstract r2" by simp
 next
   from assms(3) show "concrete r2 = abstract r3" by simp
@@ -173,27 +173,29 @@ qed
 
 (*
 lemma refinement_paths:
-assumes "sound_REFINEMENT r"
+assumes "sound_B_refinement r"
 shows "\<forall> pc \<in> lts_traces(concrete r) . \<exists> pa \<in> lts_traces(abstract r) . (invariant r) (fst pc, fst pa)"
 sorry
 *)
 
-lemma assumes "sound_REFINEMENT r" shows "lts_traces (concrete r) \<subseteq> lts_traces (abstract r)"
+lemma assumes "sound_B_refinement r" shows "lts_traces (concrete r) \<subseteq> lts_traces (abstract r)"
   sorry
 
-type_synonym DESIGN = "REFINEMENT list"
+section {* B development *}
 
-inductive sound_DESIGN :: "DESIGN \<Rightarrow> bool" where
-  base: "sound_DESIGN []" |
-  step: "\<lbrakk> sound_REFINEMENT x; xs \<noteq> [] \<longrightarrow> concrete x = abstract (hd xs) \<and> sound_DESIGN xs \<rbrakk> \<Longrightarrow> sound_DESIGN (x # xs)"
+type_synonym B_design = "B_refinement list"
+
+inductive sound_B_design :: "B_design \<Rightarrow> bool" where
+  base: "sound_B_design []" |
+  step: "\<lbrakk> sound_B_refinement x; xs \<noteq> [] \<longrightarrow> concrete x = abstract (hd xs) \<and> sound_B_design xs \<rbrakk> \<Longrightarrow> sound_B_design (x # xs)"
    
-record DEVELOPMENT =
+record B_development =
   spec :: B_machine
-  design :: DESIGN
+  design :: B_design
 
-definition sound_DEVELOPMENT :: "DEVELOPMENT \<Rightarrow> bool" where
-  "sound_DEVELOPMENT dev \<equiv> 
-    sound_B_machine (spec dev) \<and> sound_DESIGN (design dev) \<and>
+definition sound_B_development :: "B_development \<Rightarrow> bool" where
+  "sound_B_development dev \<equiv> 
+    sound_B_machine (spec dev) \<and> sound_B_design (design dev) \<and>
     (design dev \<noteq> [] \<longrightarrow> (B_machine.lts (spec dev)) = (abstract (hd (design dev))))"
     
 end
